removing the is_mutable invariants ... enhanced the FreezingArray library so that client can specify at the creation time if they never intend to freeze this array. in that case, the returned array has a witnessed stable predicate, that allows future write operations to recall the mutability. some other cleanup in the array library

examples/preorders/FreezingArray.fst
@@ -84,13 +84,17 @@ assume val copy_seq (#a:Type0) (s1:seq (option a)) (i:nat) (j:nat) (s2:seq a)
 
 (*****)
 
+private type flag =
+  | Mutable
+  | MutableUntilFrozen
+  | Frozen
+
 (*
- * representation of an array, a sequence of options and a bool, with an invariant that
- * if the bool is set, the sequence is all Some
- * the bool represents the frozen bit
+ * representation of an array, a sequence of options and a flag, with an invariant that
+ * if the flag is Frozen, the sequence is all Some
  *)
 private type repr (a:Type0) (n:nat) :Type0 =
-  t:(Seq.seq (option a) * bool){Seq.length (fst t) = n /\ (b2t (snd t) ==> (forall (i:nat). i < n ==> Some? (Seq.index (fst t) i)))}
+  t:(Seq.seq (option a) * flag){Seq.length (fst t) = n /\ ((snd t == Frozen) ==> all_some (fst t))}
 
 (*
  * relation (preorder) between sequences
@@ -98,11 +102,13 @@ private type repr (a:Type0) (n:nat) :Type0 =
  * in any case, once a sequence entry is Some, it remains Some
  *)
 private type seq_rel (a:Type0) (n:nat) :relation (repr a n)
-  = fun (t1:repr a n) (t2:repr a n) -> let s1, b1 = t1 in
-                                    let s2, b2 = t2 in
-				    (b2t b1 ==> (b2t b2 /\ (s1 == s2))) /\  //once the seq is init, it remains init
-				    (forall (i:nat). i < n ==> (Some? (Seq.index s1 i) ==>
-				                         Some? (Seq.index s2 i)))  //in any case, Some indices remain Some
+  = fun (t1:repr a n) (t2:repr a n) -> let s1, f1 = t1 in
+                                    let s2, f2 = t2 in
+				    (f1 == Mutable ==> f2 == Mutable)               /\
+				    (f1 == Frozen ==> f2 == Frozen)                 /\
+				    (f1 == MutableUntilFrozen ==> (f2 =!= Mutable)) /\
+				    (f1 == Frozen  ==> s1 == s2)                    /\  //once the seq is frozen, it remains so
+				    (forall (i:nat). i < n ==> (init_at_seq s1 i ==> init_at_seq s2 i))  //once an index is init, it remains so
 
 (* typing the relation above as preorder *)
 private let seq_pre (a:Type0) (n:nat) :preorder (repr a n) = seq_rel a n
@@ -111,84 +117,118 @@ private let seq_pre (a:Type0) (n:nat) :preorder (repr a n) = seq_rel a n
  * an array is a mref and an offset into the array (for taking interior pointers)
  * the view of an array is from offset to m
  *)
-noeq abstract type array (a:Type0) (n:nat) =
-  | A: #m:nat -> s_ref:mref (repr a m) (seq_pre a m)
-       -> offset:nat{offset + n <= m} -> array a n
+noeq abstract type t (a:Type0) (n:nat) =
+  | A: #m:nat -> s_ref:mref (repr a m) (seq_pre a m) -> offset:nat{offset + n <= m} -> t a n
+
+abstract type mutable_pred' (#a:Type0) (#n:nat) (x:t a n) :heap_predicate
+  = fun h ->
+    let A #_ #_ #_ s_ref _ = x in
+    h `Heap.contains` s_ref /\ (snd (sel h s_ref) == Mutable)
+
+abstract type mutable_pred (#a:Type0) (#n:nat) (x:t a n) :(p:heap_predicate{stable p})
+  = mutable_pred' x
+
+abstract type freezable_pred' (#a:Type0) (#n:nat) (x:t a n) :heap_predicate
+  = fun h ->
+    let A #_ #_ #_ s_ref _ = x in
+    h `Heap.contains` s_ref /\ (snd (sel h s_ref) == MutableUntilFrozen \/ (snd (sel h s_ref) == Frozen))
+
+abstract type freezable_pred (#a:Type0) (#n:nat) (x:t a n) :(p:heap_predicate{stable p})
+  = freezable_pred' x
+
+type farray (a:Type0) (n:nat) = x:t a n{witnessed (freezable_pred x)}  //an array that you intend to freeze in future
+
+type array (a:Type0) (n:nat) = x:t a n{witnessed (mutable_pred x)}  //an array that you don't intend to freeze
 
 (*
  * this is true if the current array has full view of the underlying array
  * we currently require freezing only on the full array
  *)
-abstract let is_full_array (#a:Type0) (#n:nat) (arr:array a n) :bool =
+abstract let is_full_array (#a:Type0) (#n:nat) (arr:t a n) :bool =
   let A #_ #_ #m _ off = arr in
   off = 0 && n = m
 
 (*
  * footprint of the array in the heap
  *)
-abstract let array_footprint (#a:Type0) (#n:nat) (arr:array a n) :GTot (Set.set nat)
+abstract let array_footprint (#a:Type0) (#n:nat) (arr:t a n) :GTot (Set.set nat)
   = let A s_ref _ = arr in
     Set.singleton (addr_of s_ref)
 
 (*
  * liveness of an array in the heap
  *)
-abstract let contains_array (#a:Type) (#n:nat) (h:heap) (arr:array a n)
+abstract let contains_array (#a:Type) (#n:nat) (h:heap) (arr:t a n)
   = let A #_ #_ #_ s_ref _ = arr in
     h `Heap.contains` s_ref
 
 (*
  * this is a precondition for writing, essentially, it will be false once you freeze the array
  *)
-abstract let is_mutable (#a:Type0) (#n:nat) (arr:array a n) (h:heap)
+abstract let is_mutable (#a:Type0) (#n:nat) (arr:t a n) (h:heap)
   = let A #_ s_ref _ = arr in
-    not (snd (sel h s_ref))
+    let f = snd (sel h s_ref) in
+    f == Mutable \/ f == MutableUntilFrozen
 
-let fresh_arr (#a:Type0) (#n:nat) (arr:array a n) (h0 h1:heap)
+let fresh_arr (#a:Type0) (#n:nat) (arr:t a n) (h0 h1:heap)
   = h1 `contains_array` arr /\  //array is live in h1
     (forall (n:nat). Set.mem n (array_footprint arr) ==> n `addr_unused_in` h0)  //the footprint of array was unused in h0, hopefully this enables the clients to maintain separation
 
 (*
- * create an array
+ * create an array that you intend to freeze some time in future
+ *)
+abstract let fcreate (a:Type0) (n:nat)
+  :ST (farray a n) (requires (fun _         -> True))
+                   (ensures  (fun h0 arr h1 -> fresh_arr arr h0 h1      /\  //it's fresh
+		                            modifies Set.empty h0 h1 /\  //no existing refs are changed
+					    is_mutable arr h1        /\  //the array is mutable
+					    is_full_array arr))         //and has the full view of the underlying sequence
+  = let arr = A #a #n #n (alloc ((Seq.create n None), MutableUntilFrozen)) 0 in
+    gst_witness (freezable_pred arr);
+    arr
+
+(*
+ * create an array, that always remains mutable
  *)
 abstract let create (a:Type0) (n:nat)
   :ST (array a n) (requires (fun _         -> True))
                   (ensures  (fun h0 arr h1 -> fresh_arr arr h0 h1      /\  //it's fresh
 		                           modifies Set.empty h0 h1 /\  //no existing refs are changed
-					   is_mutable arr h1        /\  //the array is mutable
 					   is_full_array arr))         //and has the full view of the underlying sequence
-  = A #a #n #n (alloc ((Seq.create n None), false)) 0
+  = let arr = A #a #n #n (alloc ((Seq.create n None), Mutable)) 0 in
+    gst_witness (mutable_pred arr);
+    arr
 
 (*
  * type of a valid index into an array
  *)
-type index (#a:Type0) (#n:nat) (arr:array a n) = i:nat{i < n}
+type index (#a:Type0) (#n:nat) (arr:t a n) = i:nat{i < n}
 
 (*
  * Ghost view of an array as a sequence of options
  *)
-abstract let as_seq (#a:Type0) (#n:nat) (arr:array a n) (h:heap)
+abstract let as_seq (#a:Type0) (#n:nat) (arr:t a n) (h:heap)
   :GTot (s:Seq.seq (option a))
   = let A #_ #_ #_ s_ref off = arr in
     let s = fst (sel h s_ref) in
     Seq.slice s off (off + n)
 
-let lemma_as_seq_length (#a:Type0) (#n:nat) (arr:array a n) (h:heap)
+let lemma_as_seq_length (#a:Type0) (#n:nat) (arr:t a n) (h:heap)
   :Lemma (requires True)
          (ensures  (Seq.length (as_seq arr h) = n))
 	 [SMTPat (Seq.length (as_seq arr h))]
   = ()
 
 (* scaffolding for init_at *)
-abstract let init_at_arr (#a:Type0) (#n:nat) (arr:array a n) (i:index arr) (h:heap) :Type0
+abstract let init_at_arr (#a:Type0) (#n:nat) (arr:t a n) (i:index arr) (h:heap) :Type0
   = let s = as_seq arr h in
     init_at_seq s i
 
-private let init_at_pred' (#a:Type0) (#n:nat) (arr:array a n) (i:index arr) :heap_predicate
+private let init_at_pred' (#a:Type0) (#n:nat) (arr:t a n) (i:index arr) :heap_predicate
   = fun h -> h `contains_array` arr /\ init_at_arr arr i h
 
 (* a stable init_at predicate *)
-abstract let init_at_pred (#a:Type0) (#n:nat) (arr:array a n) (i:index arr) :(p:heap_predicate{stable p})
+abstract let init_at_pred (#a:Type0) (#n:nat) (arr:t a n) (i:index arr) :(p:heap_predicate{stable p})
   = let A #_ #_ #m s_ref off = arr in
     assert (forall (h:heap).
               let s, _ = sel h s_ref in
@@ -201,25 +241,25 @@ abstract let init_at_pred (#a:Type0) (#n:nat) (arr:array a n) (i:index arr) :(p:
     init_at_pred' arr i
 
 (* witnessed predicate for init_at *)
-abstract let init_at (#a:Type0) (#n:nat) (arr:array a n) (i:index arr) :Type0
+abstract let init_at (#a:Type0) (#n:nat) (arr:t a n) (i:index arr) :Type0
   = witnessed (init_at_pred arr i)
 
 (* scaffolding for frozen predicate *)
-abstract let frozen_bit (#a:Type0) (#n:nat) (arr:array a n) (h:heap) :GTot bool
+abstract let frozen_bit (#a:Type0) (#n:nat) (arr:t a n) (h:heap) :Type0
   = let A s_ref _ = arr in
-    snd (sel h s_ref)
+    snd (sel h s_ref) == Frozen
 
-private type frozen_pred' (#a:Type0) (#n:nat) (arr:array a n) (s:Seq.seq a) :heap_predicate
+private type frozen_pred' (#a:Type0) (#n:nat) (arr:t a n) (s:Seq.seq a) :heap_predicate
   = fun h -> h `contains_array` arr /\ some_equivalent_seqs (as_seq arr h) s /\ frozen_bit arr h
 
 open FStar.Ghost
 
 (* a stable frozen predicate *)
-abstract type frozen_pred (#a:Type0) (#n:nat) (arr:array a n) (s:erased (Seq.seq a)) :(p:heap_predicate{stable p})
+abstract type frozen_pred (#a:Type0) (#n:nat) (arr:t a n) (s:erased (Seq.seq a)) :(p:heap_predicate{stable p})
   = frozen_pred' arr (reveal s)
 
 (* witnessed predicate for frozen *)
-abstract type frozen_with (#a:Type0) (#n:nat) (arr:array a n) (s:erased (Seq.seq a)) :Type0
+abstract type frozen_with (#a:Type0) (#n:nat) (arr:t a n) (s:erased (Seq.seq a)) :Type0
   = Seq.length (reveal s) == n /\ witnessed (frozen_pred arr s)
 
 (***** serious stuff starts now *****)
@@ -227,7 +267,7 @@ abstract type frozen_with (#a:Type0) (#n:nat) (arr:array a n) (s:erased (Seq.seq
 (*
  * freeze an array
  *)
-abstract let freeze (#a:Type0) (#n:nat) (arr:array a n)
+abstract let freeze (#a:Type0) (#n:nat) (arr:farray a n)
   :ST (s:erased (Seq.seq a))
       (requires (fun h0       -> is_full_array arr /\  //can only freeze full arrays
                               (forall (i:nat). i < n ==> init_at_arr arr i h0)))  //all elements must be init_at
@@ -235,16 +275,17 @@ abstract let freeze (#a:Type0) (#n:nat) (arr:array a n)
                               frozen_with arr es                          /\  //witnessing the stable predicate
                               (~ (is_mutable arr h1))                     /\  //the array is no longer mutable
 			      modifies (array_footprint arr) h0 h1))  //only array footprint is changed
-  = let A #_ s_ref _ = arr in
+  = gst_recall (freezable_pred arr);
+    let A #_ s_ref _ = arr in
     let s, b = !s_ref in
-    s_ref := (s, true);
+    s_ref := (s, Frozen);
     gst_witness (frozen_pred arr (hide (get_some_equivalent s)));
     hide (get_some_equivalent s)
 
 (*
  * read from an array
  *)
-abstract let read (#a:Type0) (#n:nat) (arr:array a n) (i:index arr{arr `init_at` i})  //the index must be `init_at`
+abstract let read (#a:Type0) (#n:nat) (arr:t a n) (i:index arr{arr `init_at` i})  //the index must be `init_at`
   :ST a (requires (fun h0      -> True))
         (ensures  (fun h0 r h1 -> h0 == h1 /\ Some r == Seq.index (as_seq arr h0) i))
   = let A #_ s_ref o = arr in
@@ -252,10 +293,7 @@ abstract let read (#a:Type0) (#n:nat) (arr:array a n) (i:index arr{arr `init_at`
     gst_recall (init_at_pred arr i);
     Some?.v (Seq.index s (o + i))
 
-(*
- * write into an array
- *)
-abstract let write (#a:Type0) (#n:nat) (arr:array a n) (i:nat{i < n}) (x:a)
+private let write_common (#a:Type0) (#n:nat) (arr:t a n) (i:nat{i < n}) (x:a)
   :ST unit (requires (fun h0       -> is_mutable arr h0))  //the array must be mutable
            (ensures  (fun h0 () h1 -> modifies (array_footprint arr) h0 h1 /\  //only array is modified
 	                           is_mutable arr h1                    /\  //the array remains mutable
@@ -268,17 +306,48 @@ abstract let write (#a:Type0) (#n:nat) (arr:array a n) (i:nat{i < n}) (x:a)
     gst_witness (init_at_pred arr i);
     ()
 
+abstract let write (#a:Type0) (#n:nat) (arr:array a n) (i:nat{i < n}) (x:a)
+  :ST unit (requires (fun h0       -> True))  //the array must be mutable
+           (ensures  (fun h0 () h1 -> modifies (array_footprint arr) h0 h1 /\  //only array is modified
+				   arr `init_at` i                      /\  //witness the stable init predicate
+				   Seq.index (as_seq arr h1) i == Some x))  //update the ghost view of the array
+  = gst_recall (mutable_pred arr);
+    write_common arr i x
+
+(*
+ * write into an array
+ *)
+abstract let fwrite (#a:Type0) (#n:nat) (arr:farray a n) (i:nat{i < n}) (x:a)
+  :ST unit (requires (fun h0       -> is_mutable arr h0))  //the array must be mutable
+           (ensures  (fun h0 () h1 -> modifies (array_footprint arr) h0 h1 /\  //only array is modified
+	                           is_mutable arr h1                    /\  //the array remains mutable
+				   arr `init_at` i                      /\  //witness the stable init predicate
+				   Seq.index (as_seq arr h1) i == Some x))  //update the ghost view of the array
+  = write_common arr i x
+
 (*
  * subarray
  *)
-abstract let sub (#a:Type0) (#n:nat) (arr:array a n) (i:index arr) (len:nat{i + len <= n}) :array a len
+abstract let sub (#a:Type0) (#n:nat) (arr:t a n) (i:index arr) (len:nat{i + len <= n}) :t a len
   = let A #m s_ref o = arr in
     A #m s_ref (o + i)
 
 let suffix (#a:Type0) (#n:nat) (arr:array a n) (i:index arr) = sub arr i (n - i)
 let prefix (#a:Type0) (#n:nat) (arr:array a n) (i:index arr) = sub arr 0 i
 
-let lemma_sub_is_slice (#a:Type0) (#n:nat) (arr:array a n) (i:index arr) (len:nat{i + len <= n}) (h:heap)
+let lemma_sub_preserves_array_mutable_flag (#a:Type0) (#n:nat) (arr:t a n) (i:index arr) (len:nat{i + len <= n})
+  :Lemma (requires (witnessed (mutable_pred arr)))
+         (ensures  (witnessed (mutable_pred (sub arr i len))))
+	 [SMTPat (witnessed (mutable_pred (sub arr i len)))]
+  = lemma_functoriality (mutable_pred arr) (mutable_pred (sub arr i len))
+
+let lemma_sub_preserves_array_freezable_flag (#a:Type0) (#n:nat) (arr:t a n) (i:index arr) (len:nat{i + len <= n})
+  :Lemma (requires (witnessed (freezable_pred arr)))
+         (ensures  (witnessed (freezable_pred (sub arr i len))))
+	 [SMTPat (witnessed (freezable_pred (sub arr i len)))]
+  = lemma_functoriality (freezable_pred arr) (freezable_pred (sub arr i len))
+
+let lemma_sub_is_slice (#a:Type0) (#n:nat) (arr:t a n) (i:index arr) (len:nat{i + len <= n}) (h:heap)
   :Lemma (requires True)
          (ensures  (as_seq (sub arr i len) h == Seq.slice (as_seq arr h) i (i + len)))
 	 [SMTPat (as_seq (sub arr i len) h)]
@@ -288,7 +357,7 @@ let lemma_sub_is_slice (#a:Type0) (#n:nat) (arr:array a n) (i:index arr) (len:na
  * footprint of a subarray is same as the footprint of the array
  *)
 let lemma_sub_footprint
-  (#a:Type0) (#n:nat) (arr:array a n) (i:index arr) (len:nat{i + len <= n})
+  (#a:Type0) (#n:nat) (arr:t a n) (i:index arr) (len:nat{i + len <= n})
   :Lemma (requires True)
          (ensures (let arr' = sub arr i len in
                    array_footprint arr == array_footprint arr'))
@@ -299,7 +368,7 @@ let lemma_sub_footprint
  * a subarray is live iff the array is live
  *)
 let lemma_sub_contains
-  (#a:Type0) (#n:nat) (arr:array a n) (i:index arr) (len:nat{i + len <= n}) (h:heap)
+  (#a:Type0) (#n:nat) (arr:t a n) (i:index arr) (len:nat{i + len <= n}) (h:heap)
   :Lemma (requires True)
          (ensures  (let arr' = sub arr i len in
 	            h `contains_array` arr <==> h `contains_array` arr'))
@@ -310,7 +379,7 @@ let lemma_sub_contains
  * a subarray is mutable iff the array is mutable
  *)
 let lemma_sub_is_mutable
-  (#a:Type0) (#n:nat) (arr:array a n) (i:index arr) (len:nat{i + len <= n}) (h:heap)
+  (#a:Type0) (#n:nat) (arr:t a n) (i:index arr) (len:nat{i + len <= n}) (h:heap)
   :Lemma (requires True)
          (ensures  (let arr' = sub arr i len in
 	            is_mutable arr h <==> is_mutable arr' h))
@@ -321,7 +390,7 @@ let lemma_sub_is_mutable
  * subarray of a frozen array is frozen on a subsequence of the original sequence
  *)
 let lemma_sub_frozen
-  (#a:Type0) (#n:nat) (arr:array a n) (i:index arr) (len:nat{i + len <= n}) (es:erased (Seq.seq a){frozen_with arr es})
+  (#a:Type0) (#n:nat) (arr:t a n) (i:index arr) (len:nat{i + len <= n}) (es:erased (Seq.seq a){frozen_with arr es})
   :Lemma (requires True)
          (ensures  (frozen_with (sub arr i len) (hide (Seq.slice (reveal es) i (i + len)))))
 	 [SMTPat (frozen_with arr es); SMTPat (sub arr i len)]
@@ -333,7 +402,7 @@ let lemma_sub_frozen
  * if a subarray contains an init location, it remains init
  *)
 let lemma_sub_init_at
-  (#a:Type0) (#n:nat) (arr:array a n) (i:index arr{arr `init_at` i})
+  (#a:Type0) (#n:nat) (arr:t a n) (i:index arr{arr `init_at` i})
   (j:index arr{j <= i}) (len:nat{j + len <= n /\ j + len > i})
   :Lemma (requires True)
          (ensures  ((sub arr j len) `init_at` (i - j)))
@@ -342,26 +411,26 @@ let lemma_sub_init_at
     lemma_functoriality (init_at_pred arr i) (init_at_pred arr' (i - j))
 
 (* recall various properties *)
-abstract let recall_init (#a:Type0) (#n:nat) (arr:array a n) (i:index arr{arr `init_at` i})
+abstract let recall_init (#a:Type0) (#n:nat) (arr:t a n) (i:index arr{arr `init_at` i})
   :ST unit (requires (fun _       -> True))
            (ensures  (fun h0 _ h1 -> h0 == h1 /\ Some? (Seq.index (as_seq arr h0) i)))
   = let h0 = ST.get () in
     gst_recall (init_at_pred arr i)
 
-abstract let recall_frozen (#a:Type0) (#n:nat) (arr:array a n) (es:erased (Seq.seq a){frozen_with arr es})
+abstract let recall_frozen (#a:Type0) (#n:nat) (arr:t a n) (es:erased (Seq.seq a){frozen_with arr es})
   :ST unit (requires (fun _       -> True))
            (ensures  (fun h0 _ h1 -> h0 == h1 /\ some_equivalent_seqs (as_seq arr h0) (reveal es)))
   = let h0 = ST.get () in
     gst_recall (frozen_pred arr es)
 
-abstract let recall_contains (#a:Type0) (#n:nat) (arr:array a n)
+abstract let recall_contains (#a:Type0) (#n:nat) (arr:t a n)
   :ST unit (requires (fun _       -> True))
            (ensures  (fun h0 _ h1 -> h0 == h1 /\ h0 `contains_array` arr))
   = let A #_ #_ #_ s_ref _ = arr in
     ST.recall s_ref
 
 (* frozen implies init_at at all indices *)
-let lemma_frozen_implies_init_at (#a:Type0) (#n:nat) (arr:array a n) (es:erased (Seq.seq a){frozen_with arr es}) (i:index arr)
+let lemma_frozen_implies_init_at (#a:Type0) (#n:nat) (arr:t a n) (es:erased (Seq.seq a){frozen_with arr es}) (i:index arr)
   :Lemma (requires True)
          (ensures  (arr `init_at` i))
 	 [SMTPat (frozen_with arr es); SMTPat (arr `init_at` i)]
@@ -369,24 +438,19 @@ let lemma_frozen_implies_init_at (#a:Type0) (#n:nat) (arr:array a n) (es:erased 
 
 (***** some utility functions *****)
 
-let all_init_i_j (#a:Type0) (#n:nat) (arr:array a n) (i:nat) (j:nat{j >= i /\ j <= n}) :Type0
+let all_init_i_j (#a:Type0) (#n:nat) (arr:t a n) (i:nat) (j:nat{j >= i /\ j <= n}) :Type0
   = forall (k:nat). k >= i /\ k < j ==> arr `init_at` k
 
-let all_init (#a:Type0) (#n:nat) (arr:array a n) :Type0
+let all_init (#a:Type0) (#n:nat) (arr:t a n) :Type0
   = all_init_i_j arr 0 n
 
-type iarray_i_j (a:Type0) (n:nat) (i:nat) (j:nat{j >= i /\ j <= n}) :Type0
-  = arr:array a n{all_init_i_j arr i j}
-
-type iarray (a:Type0) (n:nat) :Type0 = iarray_i_j a n 0 n
-
-let init_arr_in_heap_i_j (#a:Type0) (#n:nat) (arr:array a n) (h:heap) (i:nat) (j:nat{j >= i /\ j <= n}) :Type0
+let init_arr_in_heap_i_j (#a:Type0) (#n:nat) (arr:t a n) (h:heap) (i:nat) (j:nat{j >= i /\ j <= n}) :Type0
   = forall (k:nat). (k >= i /\ k < j) ==> init_at_seq (as_seq arr h) k
 
-let init_arr_in_heap (#a:Type0) (#n:nat) (arr:array a n) (h:heap) :Type0
+let init_arr_in_heap (#a:Type0) (#n:nat) (arr:t a n) (h:heap) :Type0
   = init_arr_in_heap_i_j arr h 0 n
 
-abstract let recall_all_init_i_j (#a:Type0) (#n:nat) (arr:array a n) (i:nat) (j:nat{j >= i /\ j <= n /\ all_init_i_j arr i j})
+abstract let recall_all_init_i_j (#a:Type0) (#n:nat) (arr:t a n) (i:nat) (j:nat{j >= i /\ j <= n /\ all_init_i_j arr i j})
   :ST unit (requires (fun _ -> True))
            (ensures  (fun h0 _ h1 -> h0 == h1 /\ init_arr_in_heap_i_j arr h0 i j))
   = let rec aux (curr:nat{curr >= i /\ curr < j})
@@ -398,12 +462,12 @@ abstract let recall_all_init_i_j (#a:Type0) (#n:nat) (arr:array a n) (i:nat) (j:
     if i = j then ()
     else aux i
 
-abstract let recall_all_init (#a:Type0) (#n:nat) (arr:array a n{all_init arr})
+abstract let recall_all_init (#a:Type0) (#n:nat) (arr:t a n{all_init arr})
   :ST unit (requires (fun _ -> True))
            (ensures  (fun h0 _ h1 -> h0 == h1 /\ init_arr_in_heap arr h0))
   = recall_all_init_i_j arr 0 n
 
-abstract let witness_all_init_i_j (#a:Type0) (#n:nat) (arr:array a n) (i:nat) (j:nat{j >= i /\ j <= n})
+abstract let witness_all_init_i_j (#a:Type0) (#n:nat) (arr:t a n) (i:nat) (j:nat{j >= i /\ j <= n})
   :ST unit (requires (fun h0      -> init_arr_in_heap_i_j arr h0 i j))
            (ensures  (fun h0 _ h1 -> h0 == h1 /\ all_init_i_j arr i j))
   = let rec aux (curr:nat{curr >= i /\ curr < j})
@@ -416,25 +480,25 @@ abstract let witness_all_init_i_j (#a:Type0) (#n:nat) (arr:array a n) (i:nat) (j
     if i = j then ()
     else aux i
 
-abstract let witness_all_init (#a:Type0) (#n:nat) (arr:array a n)
+abstract let witness_all_init (#a:Type0) (#n:nat) (arr:t a n)
   :ST unit (requires (fun h0 -> init_arr_in_heap arr h0))
            (ensures  (fun h0 _ h1 -> h0 == h1 /\ all_init arr))
   = witness_all_init_i_j arr 0 n
 
 let as_initialized_seq
-  (#a:Type0) (#n:nat) (arr:array a n) (h:heap{init_arr_in_heap arr h})
+  (#a:Type0) (#n:nat) (arr:t a n) (h:heap{init_arr_in_heap arr h})
   :GTot (seq a)
   = let s = as_seq arr h in
     get_some_equivalent s
 
-let as_initialized_subseq (#a:Type0) (#n:nat) (arr:array a n) (h:heap)
+let as_initialized_subseq (#a:Type0) (#n:nat) (arr:t a n) (h:heap)
   (i:nat) (j:nat{j >= i /\ j <= n /\ init_arr_in_heap_i_j arr h i j})
   :GTot (seq a)
   = let s = as_seq arr h in
     let s = Seq.slice s i j in
     get_some_equivalent s
 
-abstract let read_subseq_i_j (#a:Type0) (#n:nat) (arr:array a n) (i:nat) (j:nat{j >= i /\ j <= n})
+abstract let read_subseq_i_j (#a:Type0) (#n:nat) (arr:t a n) (i:nat) (j:nat{j >= i /\ j <= n})
   :ST (seq a)
       (requires (fun h0      -> all_init_i_j arr i j))
       (ensures  (fun h0 s h1 -> h0 == h1                        /\
@@ -448,7 +512,7 @@ abstract let read_subseq_i_j (#a:Type0) (#n:nat) (arr:array a n) (i:nat) (j:nat{
     let s = get_some_equivalent s in
     s
 
-abstract let fill (#a:Type0) (#n:nat) (arr:array a n) (buf:seq a{Seq.length buf <= n})
+private let fill_common (#a:Type0) (#n:nat) (arr:t a n) (buf:seq a{Seq.length buf <= n})
   :ST unit (requires (fun h0      -> is_mutable arr h0))
            (ensures  (fun h0 _ h1 -> modifies (array_footprint arr) h0 h1                   /\
 	                          all_init_i_j arr 0 (Seq.length buf)                    /\
@@ -461,22 +525,41 @@ abstract let fill (#a:Type0) (#n:nat) (arr:array a n) (buf:seq a{Seq.length buf 
     s_ref := (s1, b);
     witness_all_init_i_j arr 0 (Seq.length buf);
     lemma_get_equivalent_sequence_slice s1 off (off + Seq.length buf) buf
+
+abstract let fill (#a:Type0) (#n:nat) (arr:array a n) (buf:seq a{Seq.length buf <= n})
+  :ST unit (requires (fun h0      -> True))
+           (ensures  (fun h0 _ h1 -> modifies (array_footprint arr) h0 h1                   /\
+	                          all_init_i_j arr 0 (Seq.length buf)                    /\
+				  init_arr_in_heap_i_j arr h1 0 (Seq.length buf)         /\
+				  buf == as_initialized_subseq arr h1 0 (Seq.length buf) /\
+				  is_mutable arr h1))
+  = gst_recall (mutable_pred arr);
+    fill_common arr buf
+
+abstract let ffill (#a:Type0) (#n:nat) (arr:farray a n) (buf:seq a{Seq.length buf <= n})
+  :ST unit (requires (fun h0      -> is_mutable arr h0))
+           (ensures  (fun h0 _ h1 -> modifies (array_footprint arr) h0 h1                   /\
+	                          all_init_i_j arr 0 (Seq.length buf)                    /\
+				  init_arr_in_heap_i_j arr h1 0 (Seq.length buf)         /\
+				  buf == as_initialized_subseq arr h1 0 (Seq.length buf) /\
+				  is_mutable arr h1))
+  = fill_common arr buf
     
-let lemma_framing_of_is_mutable (#a:Type0) (#n:nat) (arr:array a n) (h0:heap) (h1:heap) (r:Set.set nat)
+let lemma_framing_of_is_mutable (#a:Type0) (#n:nat) (arr:t a n) (h0:heap) (h1:heap) (r:Set.set nat)
   :Lemma (requires (modifies r h0 h1 /\ Set.disjoint r (array_footprint arr) /\ h0 `contains_array` arr))
          (ensures  ((is_mutable arr h0 <==> is_mutable arr h1) /\
 	            (as_seq arr h0 == as_seq arr h1)))
 	 [SMTPat (modifies r h0 h1); SMTPat (is_mutable arr h0)]
   = ()
 
-let lemma_framing_of_as_seq (#a:Type0) (#n:nat) (arr:array a n) (h0:heap) (h1:heap) (r:Set.set nat)
+let lemma_framing_of_as_seq (#a:Type0) (#n:nat) (arr:t a n) (h0:heap) (h1:heap) (r:Set.set nat)
   :Lemma (requires (modifies r h0 h1 /\ Set.disjoint r (array_footprint arr) /\ h0 `contains_array` arr))
          (ensures  (as_seq arr h0 == as_seq arr h1))
 	 [SMTPat (modifies r h0 h1); SMTPat (as_seq arr h0)]
   = ()
 
 let lemma_all_init_i_j_sub
-  (#a:Type0) (#n:nat) (arr:array a n{all_init arr}) (i:index arr) (len:nat{i + len <= n})
+  (#a:Type0) (#n:nat) (arr:t a n{all_init arr}) (i:index arr) (len:nat{i + len <= n})
   :Lemma (requires True)
          (ensures  (all_init (sub arr i len)))
 	 [SMTPat (all_init arr); SMTPat (sub arr i len)]
